some extra benchmarks...

Dafny/displace.dfy
@@ -1,53 +1,58 @@
-// Status: verifier infinite loop
-
-predicate rotated(o:seq<int>, r:seq<int>) 
-requires |o| == |r|
+// Status: verifies and compiles
+// rotates a region of the array by one place forward
+predicate rotated(arr1:seq<int>, arr2:seq<int>) 
+  requires |arr1| == |arr2|
 {
-  (forall i :: 1 <= i < |o| ==> r[i] == o[i-1]) &&
-  (|o| > 0 ==> r[0] == o[|o|-1])  
+  (foldall i :: 1 <= i < |arr1| ==> arr2[i] == arr1[i - 1]) &&
+  (|arr1| > 0 ==> arr2[0] == arr1[ |arr1| - 1 ])
 }
 
-// rotates a region of the array by one place forward
 method displace(arr: array<int>, start: nat, len: nat) returns (r: array<int>)
   requires arr != null
-  requires len > 1
+  requires len > 0
   requires start + len <= arr.Length
-  // returned array is the same size as input arr
   ensures r != null && r.Length == arr.Length
-  // elements before the start of the region are unchanged
   ensures arr[..start] == r[..start]
-  // elements after the end of the rhe region are unchanged
   ensures arr[(start + len)..] == r[(start + len)..]
-  // elements in the region are skewed by one in a positive direction and wrap
-  // around
   ensures rotated(arr[start .. start+len], r[start .. start+len])
 {
   var i: nat := 0;
   r := new int[arr.Length];
-  
-  // just copy the array
-  while i < arr.Length
-    invariant i <= arr.Length
+  while i < start
+    invariant i <= start
     invariant forall k: nat :: k < i ==> r[k] == arr[k]
   {
     r[i] := arr[i];
     i := i + 1;
   }
-  assert arr[..start] == r[..start] && arr[(start + len)..] == r[(start + len)..];
   
-  i := 1;
-  r[start] := arr[start + len - 1];
+  assert arr[..start] == r[..start];
+
+  r[start] := arr[start+len-1];
   
-  // rotate the array region between start to len
-  while i < len
-    invariant 0 < i <= len
-    invariant r[..start] == arr[..start]
-    invariant r[start] == arr[start + len - 1]
-    invariant r[(start + len)..] == arr[(start + len)..]
-    invariant forall k :: 0 < k < i ==> r[start + k] == arr[start + k - 1]
+  assert r[start] == arr[start+len-1];
+  
+  i := start+1;
+  while i < start+len
+    invariant start < i <= start+len
+    invariant arr[..start] == r[..start]
+    invariant r[start] == arr[start+len-1]
+    invariant forall k: nat :: start < k < i ==> r[k] == arr[k-1]
   {
-    r[start + i] := arr[start + i - 1];
+    r[i] := arr[i-1];
     i := i + 1;
   }
+  
   assert rotated(arr[start .. start+len], r[start .. start+len]);
+  
+  i := start+len;
+  while i < arr.Length
+    invariant start+len <= i <= arr.Length
+    invariant arr[..start] == r[..start]
+    invariant rotated(arr[start .. start+len], r[start .. start+len])
+    invariant forall k: nat :: start+len <= k < i ==> r[k] == arr[k]
+  {
+    r[i] := arr[i];
+    i := i + 1;
+  }
 }
