Dafny/max.dfy
@@ -1,0 +1,11 @@
+// Status 
+
+// find maximum value of two integers
+method max(x: int,y: int) returns (r: int)
+//////////////////////////////////////////
+ensures (r == y ==> r > x) || (r == x ==> r >= y)
+{
+  // The goal is to implement, specify and verify this function!
+  if x > y { return x; }
+  return y;
+}
