Dafny/occurences.dfy
@@ -1,0 +1,24 @@
+// Status:  
+
+method occurences(items: array<int>,item: nat) returns (r: nat)
+  requires items != null
+  // some number of occurences of item
+  ensures r > 0  ==> exists k: nat :: k < items.Length && items[k] == item
+  // no occurences of item
+  ensures r == 0 ==> forall k: nat :: k < items.Length ==> items[k] != item
+{
+  var i: nat := 0;
+  var count: nat := 0;
+  
+  while i < items.Length
+    // i is increasing and there could be elements that have matched
+    invariant i <= items.Length
+    invariant count > 0  ==> exists k: nat :: k < i && items[k] == item
+    invariant count == 0 ==> forall k: nat :: k < i ==> items[k] != item
+  {
+    if items[i] == item
+      { count := count + 1; }
+    i := i + 1;
+  }
+  return count;
+}
