displace.whiley
@@ -1,40 +1,58 @@
-// Status wyc-37: verification infinite loop
-//        wyc-36: loop invariant not restored [1192ms]
-//                where all { k in 0 .. start | result[k] == arr[k] }
-//        
+// Status wyc-37: null pointer exception
+//        wyc-36: 37: loop invariant not restored
+//
 type nat is (int n) where n >= 0
 
 // rotates a region of the array by one place forward
-function displace(int[] arr, nat start, nat len) -> (int[] r)
-/////////////////////////////////////////////////////////////
-requires len > 1
-requires start + len <= |arr|
-// output array is the same size as input array
-ensures |r| == |arr|
-// all elements before the region remain the same
-ensures all { k in 0..start | r[k] == arr[k] }
-// all elements after the region remain the same
-ensures all { k in (start + len)..|arr| | r[k] == arr[k] }
-// all elements in the region are rotated by one place
-ensures all { k in start + 1..start + len | r[k] == arr[k - 1] }
-ensures r[start] == arr[start + len - 1]
+function displace( int[] arr, nat start, nat len) -> (int[] r)
+  requires len > 0
+  requires start + len <= |arr|
+  ensures |r| == |arr|
+  ensures all { k in             0..start       | r[k] == arr[k] }
+  ensures all { k in (start + len)..|arr|       | r[k] == arr[k] }
+  ensures all { k in   (start + 1)..start + len | r[k] == arr[k - 1] }
+  ensures r[start] == arr[start + len - 1]
 :
-  nat i = start + 1
-  int[] result = arr
-  assume all { k in 0..|result| | result[k] == arr[k] }
-
-  while i < (start + len)
-  ///////////////////////
-  where start < i where i <= (start + len)
-  where |result| == |arr|
-  where all { k in          0 .. start + 1 | result[k] == arr[k] }
-  where all { k in  start + 1 .. i         | result[k] == arr[k - 1] }
-  where all { k in (start+len)..|arr|      | result[k] == arr[k] }
-  :
-    result[i] = arr[i - 1]
-    i = i + 1
-
-  assert i == (start + len)
-  result[start] = arr[start + len - 1]
+  nat i = 0
+  int[] res = [0 ; |arr|]
   
-  return result
+  while i < start
+    where i <= start
+    where |res| == |arr|
+    where all { k in  0..i | res[k] == arr[k] }
+  :
+    res[i] = arr[i]
+    i = i + 1
+  
+  assert all { k in 0..start | res[k] == arr[k] }
+
+  res[start] = arr[start + len - 1]
+  
+  assert res[start] == arr[start + len - 1]
+  
+  i = start + 1
+  while i < start + len
+    where |res| == |arr|
+    where start < i && i <= (start + len)
+    where res[start] == arr[start + len - 1]
+    where all { k in           0..start | res[k] == arr[k] }
+    where all { k in (start + 1)..i     | res[k] == arr[k - 1] }
+  :
+    res[i] = arr[i - 1]
+    i = i + 1
+  
+  assert all { k in (start + 1)..start + len | res[k] == arr[k - 1] }
+  
+  i = start + len
+  while i < |arr|
+    where |res| == |arr|
+    where (start + len) <= i && i <= |arr|
+    where res[start] == arr[start + len - 1]
+    where all { k in             0..start       | res[k] == arr[k] }
+    where all { k in   (start + 1)..start + len | res[k] == arr[k - 1] }
+    where all { k in (start + len)..i           | res[k] == arr[k] }
+  :
+    res[i] = arr[i]
+    i = i + 1
+  
+  return res
