firstIndexOf.whiley
@@ -1,0 +1,23 @@
+// Status wyc-37: 
+//        wyc-36: 
+
+function firstIndexOf(int[] items, int item) -> (int r)
+// If result is positive, element at that position must match item
+ensures r >= 0 ==> items[r] == item
+// If result is positive, no element at lesser position matches item
+ensures r >= 0 ==> all { k in 0..r | items[k] != item }
+// If result is negative, no element matches item
+ensures r <  0 ==> no  { k in 0..|items| | items[k] == item }
+:
+  int i = 0
+  while i < |items|
+  // i is increasing and no element at greater position matches item
+  where 0 <= i && i <= |items|
+  where no { k in 0..i | items[k] == item }
+  :
+    i = i + 1
+    if items[i] == item
+    :
+      return i
+  // didn't find item in entire list
+  return -1 
