max.whiley
@@ -1,0 +1,12 @@
+// Status wyc-37: .
+//        wyc-36: .
+
+// find maximum value of two integers
+public function max(int x, int y) -> (int r)
+////////////////////////////////////////////
+ensures (r == y ==> r > x) || (r == x ==> r >= y)
+:
+  // The goal is to implement, specify and verify this function!
+  if x > y:
+    return x
+  return y
