maxArray.whiley
@@ -1,0 +1,21 @@
+// Status wyc-37: verifies [1745ms]. ~228.48% improvment
+//        wyc-36: verifies [3987ms].
+
+// Append a single item onto the end of the array
+public function maxArray(int[] items) -> (int max)
+//////////////////////////////////////////////////
+requires |items| > 0
+ensures some { k in 0..|items| | max >= items[k] }
+:
+  // The goal is to implement, specify and verify this function!
+  int i = 1
+  int r = items[0]
+  //
+  while i < |items|
+  where 0 < i && i <= |items| 
+  :
+      if items[i] > r:
+        items[i] = r
+      i = i + 1
+  //
+  return r
